src/sem/Farcall.v
@@ -397,7 +397,7 @@ Definition select_ctx type (reg_ctx frame_ctx: u128) :=
 
 (* Not implemented yet: shards *)
 Inductive farcall (type:farcall_type) dest_addr handler_addr call_as_static abi_ptr_tag: FarCall.params -> state -> state -> Prop :=
-| farcall_fwd_fatptr: forall flags old_regs old_pages xstack0 xstack1 xstack2 new_caller_stack depot codes reg_context_u128 new_pages new_code_page new_mem_ctx in_ptr __ ergs_query ergs_actual fwd_mode is_syscall_query out_ptr,
+| farcall_fwd_fatptr: forall flags old_regs old_pages xstack0 xstack1 xstack2 new_caller_stack gs reg_context_u128 new_pages new_code_page new_mem_ctx in_ptr __ ergs_query ergs_actual fwd_mode is_syscall_query out_ptr,
     let old_extframe := topmost_extframe xstack0 in
     let mem_ctx0 := old_extframe.(ecf_pages) in
     let current_contract := old_extframe.(ecf_this_address) in
@@ -406,7 +406,7 @@ Inductive farcall (type:farcall_type) dest_addr handler_addr call_as_static abi_
 
     abi_ptr_tag = true ->
     
-    paid_code_fetch allow_masking depot codes dest_addr xstack0 (xstack1, new_code_page) ->
+    paid_code_fetch allow_masking gs.(gs_depot) gs.(gs_contracts) dest_addr xstack0 (xstack1, new_code_page) ->
     paid_forward Ret.ForwardFatPointer (in_ptr, xstack1) (out_ptr, xstack2) ->
     alloc_pages_extframe (old_pages,mem_ctx0) new_code_page (new_pages, new_mem_ctx) ->
     pass_allowed_ergs (ergs_query,xstack2) (ergs_actual, new_caller_stack) ->
@@ -419,7 +419,7 @@ Inductive farcall (type:farcall_type) dest_addr handler_addr call_as_static abi_
                          ecf_code_address := zero16;
                          ecf_pages := new_mem_ctx;
                          ecf_is_static :=  ecf_is_static old_extframe || call_as_static;
-                         ecf_saved_depot := depot;
+                         ecf_saved_depot := gs.(gs_depot);
                          ecf_common := {|
                                         cf_exception_handler_location := handler_addr;
                                         cf_sp := INITIAL_SP_ON_FAR_CALL;
@@ -445,8 +445,7 @@ Inductive farcall (type:farcall_type) dest_addr handler_addr call_as_static abi_
               gs_context_u128 := reg_context_u128;
 
 
-              gs_depot        := depot;
-              gs_contracts    := codes;
+              gs_global       := gs;
             |}
             {|
               gs_flags        := flags_clear;
@@ -456,16 +455,15 @@ Inductive farcall (type:farcall_type) dest_addr handler_addr call_as_static abi_
               gs_context_u128 := zero128;
 
 
-              gs_depot        := depot;
-              gs_contracts    := codes;
+              gs_global       := gs;
             |}
-| farcall_fwd_memory: forall flags old_regs old_pages xstack0 xstack1 xstack2 new_caller_stack depot codes reg_context_u128 new_pages new_code_page new_mem_ctx in_ptr __ ergs_query ergs_actual is_syscall_query out_ptr page_type,
+| farcall_fwd_memory: forall gs flags old_regs old_pages xstack0 xstack1 xstack2 new_caller_stack reg_context_u128 new_pages new_code_page new_mem_ctx in_ptr __ ergs_query ergs_actual is_syscall_query out_ptr page_type,
     let old_extframe := topmost_extframe xstack0 in
     let current_contract := old_extframe.(ecf_this_address) in
     let is_system := addr_is_kernel dest_addr && is_syscall_query in
     let allow_masking := negb is_system in
 
-    paid_code_fetch allow_masking depot codes dest_addr xstack0 (xstack1, new_code_page) ->
+    paid_code_fetch allow_masking gs.(gs_depot) gs.(gs_contracts) dest_addr xstack0 (xstack1, new_code_page) ->
     paid_forward (Ret.UseMemory page_type) (in_ptr, xstack1) (out_ptr, xstack2) ->
     
     let mem_ctx1 := (topmost_extframe xstack2).(ecf_pages) in
@@ -480,7 +478,7 @@ Inductive farcall (type:farcall_type) dest_addr handler_addr call_as_static abi_
                          ecf_code_address := zero16;
                          ecf_pages := new_mem_ctx;
                          ecf_is_static :=  ecf_is_static old_extframe || call_as_static;
-                         ecf_saved_depot := depot;
+                         ecf_saved_depot := gs.(gs_depot);
                          ecf_common := {|
                                         cf_exception_handler_location := handler_addr;
                                         cf_sp := INITIAL_SP_ON_FAR_CALL;
@@ -506,8 +504,7 @@ Inductive farcall (type:farcall_type) dest_addr handler_addr call_as_static abi_
               gs_context_u128 := reg_context_u128;
 
 
-              gs_depot        := depot;
-              gs_contracts    := codes;
+              gs_global       := gs;
             |}
             {|
               gs_flags        := flags_clear;
@@ -516,9 +513,7 @@ Inductive farcall (type:farcall_type) dest_addr handler_addr call_as_static abi_
               gs_callstack    := new_stack;
               gs_context_u128 := zero128;
 
-
-              gs_depot        := depot;
-              gs_contracts    := codes;
+              gs_global       := gs;
             |}
 .
 
